\documentclass[10.5pt]{article}
\usepackage{amsmath, amsfonts, amssymb,amsthm}
\usepackage[includeheadfoot]{geometry} % For page dimensions
\usepackage{fancyhdr}
\usepackage{enumerate} % For custom lists
\usepackage{tikz-cd}
\usepackage{graphicx}

\fancyhf{}
\lhead{MAT1301 hw1}
\rhead{Tighe McAsey - 1008309420}
\pagestyle{fancy}

% Page dimensions
\geometry{a4paper, margin=1in}

\theoremstyle{definition}
\newtheorem{pb}{}
\usepackage{tikz-cd, stackengine}

% Commands:

\newcommand{\set}[1]{\{#1\}}
\newcommand{\gen}[1]{\langle#1\rangle}
\newcommand{\abs}[1]{\left\vert#1\right\vert}
\newcommand{\norm}[1]{\lvert\lvert#1\rvert\rvert}
\newcommand{\tand}{\text{ and }}
\newcommand{\tor}{\text{ or }}
\newcommand{\pd}{\frac{\partial}{\partial x_j}}
\newcommand{\px}{\frac{\partial}{\partial x}}
\newcommand{\py}{\frac{\partial}{\partial y}}
\newcommand{\pz}{\frac{\partial}{\partial z}}
\newcommand{\ppx}{\frac{\partial^2}{\partial x^2}}
\newcommand{\ppy}{\frac{\partial^2}{\partial y^2}}
\newcommand{\ppz}{\frac{\partial^2}{\partial z^2}}
\newcommand{\hess}{\operatorname{Hess}}

\begin{document}
\begin{pb}
    \begin{align*}
        h(t,s) = \begin{cases}
            \gamma(2t) & t \leq \frac{1 - s}{2} \\
            \gamma\left(1-s\right) & t \in \left(\frac{1 - s}{2},\frac{1 + s}{2}\right) \\
            \overline{\gamma}(2(t-\frac12)) & t \geq \frac{1 + s}{2}
        \end{cases}
    \end{align*} \qed
\end{pb}
\begin{pb}
    \textbf{((iii) \(\mathbf{\implies}\) (i)):} Apply problem 3, in particular any element \([f] \in \pi_1(X,x_0)\) satisfies
    \begin{align*}
        [f] = [\alpha][1_{x_0}][\alpha]^{-1} = [1_{x_0}]
    \end{align*}

    \textbf{((i) \(\mathbf{\implies}\) (iii)):} Apply problem 3, since there is only one conjugacy class of \(\pi_1(X,x_0)\) there is only one homotopy class \(S^1 \to X\). Alternatively, let \(f_1, f_2: S^1 \to X\), where we parameterize \(S_1\) as \(\frac{I}{0\sim 1}\), since \(X\) is path connected, there is some path \(\gamma: I \to X\) with \(\gamma(0) = f_1(0) \tand \gamma(1) = f_2(0)\), then by assumption (i), \([f_1] = [1_{f_1(0)}]\) and \([f_2] = [1_{f_2(0)}]\), now we can write the homotopy between \(1_{f_1(0)} \sim f_1\) and \(1_{f_2(0)} \sim f_2\), which is given by \(h(s,t) = \gamma(s)\). \qed

    \textbf{((ii) \(\mathbf{\implies}\) (i)):} Let \([\gamma] \in \pi_1(X,x_0)\) for some \(x_0 \in X\), then we can define new paths
    \begin{align*}
        &\gamma_1: t \mapsto \gamma(t/2) &\gamma_2: t \mapsto \gamma\left(\frac{1 + t}{2}\right)
    \end{align*}
    then \(\overline{\gamma_1}\) and \(\gamma_2\) satisfy the hypotheses of (ii), which entails \(\gamma_2 \sim \overline{\gamma_1}\), now since \(\gamma = \gamma_1 \cdot \gamma_2\) we find that \(\gamma \sim \gamma_1\cdot \overline{\gamma_1} \sim 1_{x_0}\), whence \([\gamma] = [1_{x_0}]\). Since \([\gamma]\) was arbitrary we conclude \(\pi_1(X,x_0) = 0\). \qed

    \textbf{((i) \(\mathbf{\implies}\) (ii)):} Let \(f,g: I \to X\) with \(x = f(0) = g(0) \tand y = f(1) = g(1)\), then from (i) we get a homotopy \(h\) witnessing \(f \overline{g} \sim 1_x\), moreover there is some homotopy \(r\) giving \(\overline{g} g \sim 1_y\) satisfying \(h(1,s) = h(0,s) = x\) for all \(s\), and \(r(1,s) = r(0,s) = y\) for all \(s\). It is clearly sufficient to provide some path \(\gamma\) such that \(f\) is homotopic to \(\gamma\) by \(h'\) without moving endpoints, and same for \(g\) by \(h''\), since then the following homotopy satisfies the desideratum
    \begin{align*}
        H(t,s) = \begin{cases}
            h'(t,2s) & s \in [0,\frac12] \\
            h''(1-t,1 - 2(s - \frac12)) & s \in (\frac12,1]
        \end{cases}
    \end{align*}
    Taking \(\gamma = f \overline{g}g\), we find that \(h'\) can be taken to be
    \begin{align*}
        h'(t,s) = \begin{cases}
            h(2t,s) & t \in [0,\frac12] \\
            g(2(t-\frac12)) & t \in (\frac12,1]
        \end{cases}
    \end{align*}
    and \(h''\) can be taken to be
    \begin{align*}
       h''(t,s) =  \begin{cases}
            f(2t) & t \in [0,\frac12] \\
        r(s,2(t-\frac12)) & t \in (\frac12,1]
        \end{cases}
    \end{align*}
    \qed
\end{pb}
\begin{pb}
    Define the map
    \begin{align*}
        \psi: \pi_1(X,x_0) &\to \set{S^1 \to X}/\sim \\
            [f] &\mapsto [f]
    \end{align*}
    In words, we forget the base point of \(f\). This is of course well defined up to homotopy. To check it is well defined on conjugacy classes, it suffices to check that \([f] = [\alpha][f][\alpha]^{-1}\) for arbitrary \(f\) and \(\alpha\). This is straightforward by choosing the representative with \(\alpha\), \(f\) and \(\bar{\alpha}\) each being sped up by \(3\) times, and defining the homotopy
    \begin{align*}
        h(t,s) = \begin{cases}
            \alpha(s + 3t) & t \leq \frac{1-s}{3}\\
            f(\frac{t - \frac{1-s}{3}}{1-2\frac{1-s}{3}}) & t \in (\frac{1-s}{3},\frac{2+s}{3})\\
            \alpha(1+s - 3(t - \frac23)) & t \geq \frac{2+s}{3}
        \end{cases}
    \end{align*}
    
    To see that this map is onto, it suffices to check that every map \(f: S^1 \to X\) is homotopic to a map \(f'\) with \(f'(0) = x_0\). Now checking this consider some \(f: S^1 \to X\), and let \(\gamma\) be a path between \(x_0\) and \(f(0)\), then we can write
    \begin{align*}
        f'(t) = \begin{cases}
            \gamma(3t) & t \leq \frac13 \\
            f(3(t - \frac13)) & t \in (\frac13,\frac23) \\
            \gamma(1 - 3(t - \frac23)) & t \geq \frac23
        \end{cases}
    \end{align*}
    Then we can verify explicitly that \(f' \sim f\)
    \begin{align*}
        h'(t,s) = \begin{cases}
            \gamma(s + 3t) & t \leq \frac{1-s}{3}\\
            f(\frac{t - \frac{1-s}{3}}{1-2\frac{1-s}{3}}) & t \in (\frac{1-s}{3},\frac{2+s}{3})\\
            \gamma(1+s - 3(t - \frac23)) & t \geq \frac{2+s}{3}
        \end{cases}
    \end{align*}
    Finally, we need to check injectivity. Assume that \(\psi([f]) = \psi([g])\), then there is some homotopy \(h: S^1 \times I \to X\) witnessing this equivalence, then we can define \(\alpha(s) = h(0,s) = h(1,s)\). It remains to check that \([\alpha][f][\alpha]^{-1} = [g]\), this equivalence is given by the following (based) homotopy between \([\alpha][f][\alpha]^{-1}\) and \([1_{x_0}][f][1_{x_0}] = [f]\).
    \begin{align*}
        H(t,s) = \begin{cases}
            h(0,3(1-s)t) & t \leq \frac13 \\
            h(3(t-\frac13),1-s) & t \in  (\frac13,\frac23)\\
            h(1,(1-s)-3(1-s)(t-\frac23)) & t \geq \frac23
        \end{cases}
    \end{align*}
    \qed
\end{pb}
\end{document}